\documentclass[12pt]{article}
 
\usepackage[margin=1in]{geometry} 
\usepackage{amsmath,amsthm,amssymb}
\usepackage{graphicx}
 
\newcommand{\N}{\mathbb{N}}
\newcommand{\Z}{\mathbb{Z}}
\newcommand{\R}{\mathbb{R}}
\newcommand{\C}{\mathbb{C}}
 
 
\begin{document}


\title{Solutions to Sheet 3}
\author{Lukas Drexler, Leif Van Holland \\ \\
\textsc{Pattern Matching and Machine Learning} \\
\textsc{for Audio Signal Processing}}
\maketitle

\section*{Exercise 3.1}
\begin{itemize}
    \item[a)] \begin{align*}
        X_0 = \left(\omega_N^{0\cdot 0},\: ...\:, \omega_N^{0\cdot (N-1)}\right)\cdot x
        &=\sum_{k=0}^{N-1} \underbrace{\omega_N^0}_{=1}\cdot x_k
        = \sum_{k=0}^{N-1} x_k \in \R \\
        \\
        X_M = \left(\omega_N^{0M},\: ...\:, \omega_N^{(N-1)M}\right)\cdot x
        &= \sum_{k=0}^{N-1}\omega_N^{k M}\cdot x_k
        = \sum_{k=0}^{N-1}\exp\left(\frac{-2\pi i M}{2M}\right)^k\cdot x_k \\
        &= \sum_{k=0}^{N-1}\exp(-\pi i k)\cdot x_k = \sum_{k=0}^{N-1} (-1)^k \cdot x_k \in \R \\
        \\
        X_{N-k} = \sum_{l=0}^{N-1} \omega_N^{l(N-k)}\cdot x_l 
        &= \sum_{l=0}^{N-1} \exp\left(\frac{-2\pi i l (N-k)}{N}\right)\cdot x_l \\
        &= \sum_{l=0}^{N-1} \exp\left(\frac{2\pi i\cdot l k}{N} - 2\pi i\cdot l N\right)\cdot x_l \\
        &= \sum_{l=0}^{N-1} \exp\left(\frac{2\pi i\cdot l k}{N} \right) \underbrace{\exp(2\pi i\cdot l N)}_{=1}\cdot x_l \\
        &= \sum_{l=0}^{N-1} \overline{\exp\left(\frac{-2\pi i \cdot l k}{N}\right)\cdot x_l} \\
        &= \sum_{l=0}^{N-1} \overline{\omega_N^{lk} \cdot x_l} = \overline{X_k}
    \end{align*}
\end{itemize}

\section*{Exercise 3.2}
For $x=(2,3,-1,1)$ we get
\begin{align*}
    X_0 &= \sum_{k=0}^3 \omega_4^{0\cdot k} \cdot x_k
    = \sum_{k=0}^3 x_k = 5 \\ \\
    X_1 &= \sum_{k=0}^3 \omega_4^k\cdot x_k
    = \sum_{k=0}^3 \exp\left(\frac{-2\pi i k}{N}\right)\cdot x_k \\
    &= x_0 - i\cdot x_1 + x_2 - i\cdot x_3
    = 2 - 3i + 1 + i = 3 - 2i \\ \\
    X_2 &= \sum_{k=0}^3 \omega_4^{2k}\cdot x_k
    = x_0 - x_1 + x_2 - x_3 = 2-3-1-1 = -3 \\ \\
    X_3 &= \overline{X_1} = 3 + 2i
\end{align*}
All in all, $X = (5, 3-2i, -3, 3+2i)^T.$

\end{document}